keep working on stuff

src/indexing.v
@@ -9,6 +9,7 @@ From stdpp Require Import sets.
 From stdpp Require Import list.
 Require Import Burrow.gmap_utils.
 Require Import Burrow.rollup.
+Require Import coq_tricks.Deex.
 
 Definition PathLoc : Type := list nat * nat.
 Definition plend (pl: PathLoc) := match pl with (_, l) => l end.
@@ -21,27 +22,25 @@ Context {refinement_of_index : RefinementIndex -> Refinement M M}.*)
 
 Context {M} `{!EqDecision M, !TPCM M}.
 
-Fixpoint branch_step_branch (branch: Branch M) (idx: nat) :=
-  match branch, idx with
-  | BranchNil, _ => BranchNil
-  | BranchCons _ sub, (S idx) => branch_step_branch sub idx
-  | BranchCons (CellNode _ b) _, 0 => b
-  end.
-  
 Definition triv_cell : Cell M := CellCon unit empty.
 Definition triv_node : Node M := CellNode triv_cell BranchNil.
 
-Fixpoint branch_step_node (branch: Branch M) (idx: nat) :=
+Fixpoint step_node (branch: Branch M) (idx: nat) :=
   match branch, idx with
   | BranchNil, _ => triv_node
-  | BranchCons _ sub, (S idx) => branch_step_node sub idx
+  | BranchCons _ sub, (S idx) => step_node sub idx
   | BranchCons n _, 0 => n
+  end.
+
+Definition step_branch (branch: Branch M) (idx: nat) :=
+  match step_node branch idx with
+  | CellNode _ b => b
   end.
   
 Fixpoint node_of_pl' (branch: Branch M) (p: list nat) (i: nat) : Node M :=
   match p with
-  | [] => branch_step_node branch i
-  | (x :: p0) => node_of_pl' (branch_step_branch branch x) p0 i
+  | [] => step_node branch i
+  | (x :: p0) => node_of_pl' (step_branch branch x) p0 i
   end.
   
 Definition node_of_pl (branch: Branch M) (pl: PathLoc) : Node M :=
@@ -65,48 +64,120 @@ Lemma every_node_equiv_forall {M} `{!EqDecision M, !TPCM M}
 Lemma node_trivial_triv_node : node_trivial triv_node.
 Proof. unfold node_trivial, triv_node, cell_trivial, triv_cell. crush.
 Qed.
-  
-Lemma branch_step_node_op branch1 branch2 i
-  : branch_step_node branch1 i ⋅ branch_step_node branch2 i
-      ≡ branch_step_node (branch1 ⋅ branch2) i.
+
+Lemma node_trivial_step_node : ∀ i branch ,
+  (branch_trivial branch) -> node_trivial (step_node branch i).
+Proof.
+  induction i.
+  - intros. unfold node_trivial, step_node; destruct branch; trivial.
+    + destruct H. trivial.
+    + apply node_trivial_triv_node.
+  - intros. unfold step_node. unfold node_trivial; destruct branch; trivial.
+    + apply IHi. destruct H; trivial.
+    + apply node_trivial_triv_node.
+Qed.
+
+Lemma step_node_equiv branch1 branch2 i
+  (equ: branch1 ≡ branch2) : step_node branch1 i ≡ step_node branch2 i.
+Proof.
+  generalize equ. generalize branch1, branch2. clear equ. clear branch1. clear branch2.
+  induction i.
+  - intros. unfold step_node. destruct branch1, branch2.
+    + unfold "≡", branch_equiv in equ. destruct_ands; trivial.
+    + unfold "≡" in *. unfold branch_equiv, node_equiv in *.
+        unfold branch_trivial in equ. destruct_ands. apply node_equiv_of_trivial; trivial.
+        apply node_trivial_triv_node.
+    + unfold "≡" in *. unfold branch_equiv in *. unfold branch_trivial in equ.
+        destruct_ands. apply node_equiv_of_trivial; trivial.
+        apply node_trivial_triv_node.
+    + trivial.
+  - intros. unfold step_node. destruct branch1, branch2.
+    + apply IHi. destruct equ. trivial.
+    + apply node_equiv_of_trivial.
+      * fold step_node. apply node_trivial_step_node. destruct equ. trivial.
+      * apply node_trivial_triv_node.
+    + apply node_equiv_of_trivial.
+      * apply node_trivial_triv_node.
+      * fold step_node. apply node_trivial_step_node. destruct equ. trivial.
+    + trivial.
+Qed.
+
+Global Instance step_node_equiv_proper : Proper ((≡) ==> (=) ==> (≡)) step_node.
+Proof. unfold Proper, "==>". intros. rewrite H0. apply step_node_equiv. trivial. Defined.
+
+Lemma step_branch_equiv branch1 branch2 i
+  (equ: branch1 ≡ branch2) : step_branch branch1 i ≡ step_branch branch2 i.
+Proof.
+  assert (step_node branch1 i ≡ step_node branch2 i) by (apply step_node_equiv; trivial).
+  unfold step_branch. destruct (step_node branch1 i).
+      destruct (step_node branch2 i).
+      unfold "≡", node_equiv in H. destruct_ands; trivial.
+Qed.
+
+Global Instance step_branch_equiv_proper : Proper ((≡) ==> (=) ==> (≡)) step_branch.
+Proof. unfold Proper, "==>". intros. rewrite H0. apply step_branch_equiv. trivial. Defined.
+
+Definition node_of_pl'_equiv p : ∀ branch1 branch2 i ,
+  (branch1 ≡ branch2) -> node_of_pl' branch1 p i ≡ node_of_pl' branch2 p i.
+  induction p.
+   - unfold node_of_pl'. apply step_node_equiv.
+   - unfold node_of_pl'. fold node_of_pl'. intros.
+      apply IHp. apply step_branch_equiv. trivial.
+Qed.
+
+Global Instance node_of_pl'_proper : Proper ((≡) ==> (=) ==> (=) ==> (≡)) node_of_pl'.
+Proof. unfold Proper, "==>". intros. rewrite H1. rewrite H0. apply node_of_pl'_equiv. trivial. Defined.
+
+Definition node_of_pl_equiv : ∀ branch1 branch2 pl ,
+  (branch1 ≡ branch2) -> node_of_pl branch1 pl ≡ node_of_pl branch2 pl.
+Proof. intros. unfold node_of_pl. destruct pl. apply node_of_pl'_equiv. trivial. Qed.
+
+Global Instance node_of_pl_proper : Proper ((≡) ==> (=) ==> (≡)) node_of_pl.
+Proof. unfold Proper, "==>". intros. rewrite H0. apply node_of_pl_equiv. trivial. Defined.
+
+Lemma step_node_op branch1 branch2 i
+  : step_node branch1 i ⋅ step_node branch2 i
+      ≡ step_node (branch1 ⋅ branch2) i.
 Proof.
   generalize branch1, branch2. clear branch1. clear branch2.
   induction i.
-  - intros. unfold "⋅", node_op, branch_op, branch_step_node. destruct branch1, branch2.
+  - intros. unfold "⋅", node_op, branch_op, step_node. destruct branch1, branch2.
      + unfold "⋅". trivial.
      + apply op_trivial_node. apply node_trivial_triv_node.
      + setoid_rewrite node_op_comm.
        apply op_trivial_node. apply node_trivial_triv_node.
      + apply op_trivial_node. apply node_trivial_triv_node.
-  - intros. unfold "⋅", node_op, branch_op, branch_step_node. destruct branch1, branch2.
-     + fold branch_step_node. fold node_op. apply IHi.
-     + fold branch_step_node. fold node_op.
+  - intros. unfold "⋅", node_op, branch_op, step_node. destruct branch1, branch2.
+     + fold step_node. fold node_op. apply IHi.
+     + fold step_node. fold node_op.
         setoid_rewrite op_trivial_node; trivial. apply node_trivial_triv_node.
-     + fold branch_step_node. fold node_op.
+     + fold step_node. fold node_op.
         setoid_rewrite node_op_comm.
         setoid_rewrite op_trivial_node; trivial. apply node_trivial_triv_node.
-     + fold branch_step_node. fold node_op.
+     + fold step_node. fold node_op.
         setoid_rewrite op_trivial_node; trivial. apply node_trivial_triv_node.
 Qed.
 
-Lemma branch_step_branch_op branch1 branch2 i
-  : branch_step_branch branch1 i ⋅ branch_step_branch branch2 i
-      ≡ branch_step_branch (branch1 ⋅ branch2) i.
+Lemma step_branch_op branch1 branch2 i
+  : step_branch branch1 i ⋅ step_branch branch2 i
+      ≡ step_branch (branch1 ⋅ branch2) i.
 Proof.
+  unfold step_branch. 
+  
   generalize branch1, branch2. clear branch1. clear branch2.
   induction i.
-  - intros. unfold "⋅". unfold branch_op, branch_step_node. destruct branch1, branch2.
-     + fold branch_op. unfold branch_step_branch. destruct n. destruct n0. unfold "⋅".
+  - intros. unfold "⋅". unfold branch_op, step_node. destruct branch1, branch2.
+     + fold branch_op. unfold step_branch. destruct n. destruct n0. unfold "⋅".
         trivial.
-     + fold branch_op. cbn [branch_step_branch]. destruct n. apply op_trivial_branch.
+     + fold branch_op. cbn [step_branch]. destruct n. apply op_trivial_branch.
         unfold branch_trivial. trivial.
-     + fold branch_op. cbn [branch_step_branch]. destruct n. unfold branch_op. trivial.
-     + fold branch_op. cbn [branch_step_branch]. unfold branch_op. trivial.
-  - intros. unfold "⋅". unfold node_op, branch_op, branch_step_branch. destruct branch1, branch2.
-     + destruct n. destruct n0. fold branch_op. fold branch_step_branch. fold node_op. unfold "⋅". unfold node_op. apply IHi.
-     + destruct n. fold branch_op. fold branch_step_branch.
+     + fold branch_op. cbn [step_branch]. destruct n. unfold branch_op. trivial.
+     + fold branch_op. cbn [step_branch]. unfold branch_op. trivial.
+  - intros. unfold "⋅". unfold node_op, branch_op, step_branch. destruct branch1, branch2.
+     + destruct n. destruct n0. fold branch_op. fold step_branch. fold node_op. unfold "⋅". unfold node_op. apply IHi.
+     + destruct n. fold branch_op. fold step_branch.
         setoid_rewrite op_trivial_branch; trivial. unfold branch_trivial. trivial.
-     + destruct n. fold branch_op. fold branch_step_branch. trivial.
+     + destruct n. fold branch_op. fold step_branch. trivial.
      + trivial.
 Qed.
 
@@ -116,10 +187,10 @@ Proof.
   generalize branch1, branch2. clear branch1. clear branch2.
   destruct pl. rename l into p. rename n into i.
   induction p.
-  - intros. unfold node_of_pl, node_of_pl'. apply branch_step_node_op.
+  - intros. unfold node_of_pl, node_of_pl'. apply step_node_op.
   - intros.
       unfold node_of_pl in *. cbn [node_of_pl'].
-      setoid_rewrite <- branch_step_branch_op.
+      setoid_rewrite <- step_branch_op.
   
 
 Lemma cell_of_pl_op {M} `{!EqDecision M, !TPCM M}
